namespaces and stuff

src/computational_monads/simulation_semantics/constructions/tracking_oracle.lean
@@ -3,17 +3,12 @@ import computational_monads.simulation_semantics.simulate
 open oracle_comp oracle_spec
 
 variables {A B : Type} {spec spec' spec'' : oracle_spec}
-  (oa : oracle_comp spec A)
-
--- TODO: use namespaces to simplify the lemma names
-
--- TODO: should be able to use `simps` everywhere instead of implementing projections
 
 /-- Oracle where the query result is indepenent of the current oracle state,
   although the new state may depend upon the previous state.
   For example a logging oracle that just tracks the input and output of queries. -/
 @[simps]
-def tracking_oracle {S : Type} (default_state : S)
+def tracking_oracle {spec : oracle_spec} {S : Type} (default_state : S)
   (o : Π (i : spec.ι), spec.domain i → oracle_comp spec' (spec.range i))
   (update_state : Π (s : S) (i : spec.ι), spec.domain i → spec.range i → S) :
   simulation_oracle spec spec' :=
@@ -24,13 +19,30 @@ def tracking_oracle {S : Type} (default_state : S)
 notation `⟪` o `|` update_state `,` default_state `⟫` :=
   tracking_oracle default_state o update_state
 
+namespace tracking_oracle
+
+variables (oa : oracle_comp spec A)
+
 variables {S : Type} (default_state : S)
   (o : Π (i : spec.ι), spec.domain i → oracle_comp spec' (spec.range i))
   (update_state : Π (s : S) (i : spec.ι), spec.domain i → spec.range i → S)
 
+lemma apply (i : spec.ι) (t : spec.domain i) (s : S) :
+  ⟪o | update_state, default_state⟫.o i (t, s) =
+    do { u ← o i t, pure (u, update_state s i t u) } := rfl
+
+section simulate
+
+
+end simulate
+
+section eval_distribution
+
+variable [spec.finite_range]
+
 -- TODO: should be able to find some generalization for lemmas looking like this
-lemma simulate'_tracking_oracle_query_equiv [spec.finite_range]
-  (s : S) : simulate' (⟪query | update_state, default_state⟫) oa s ≃ₚ oa :=
+lemma simulate'_query_equiv (s : S) :
+  simulate' (⟪query | update_state, default_state⟫) oa s ≃ₚ oa :=
 begin
   induction oa with A a A B oa ob hoa hob i t generalizing s,
   { simp only [pure'_eq_pure, simulate'_pure, pure_map_equiv, eval_distribution_return] },
@@ -43,3 +55,7 @@ begin
   { erw [simulate'_query_equiv, tracking_oracle_o,
       fst_map_bind_mk_equiv, map_id_equiv (query i t)], } 
 end
+
+end eval_distribution
+
+end tracking_oracle
