src/computational_monads/simulation_semantics/constructions/identity_oracle.lean
@@ -3,16 +3,14 @@ import computational_monads.simulation_semantics.constructions.stateless_oracle
 open oracle_comp oracle_spec
 
 variables {A B : Type} {spec spec' spec'' : oracle_spec}
-  (oa : oracle_comp spec A)
 
+@[simps]
 def identity_oracle (spec : oracle_spec) : simulation_oracle spec spec :=
 ⟪ query ⟫
 
 notation `idₛ` := identity_oracle _
 
-@[simp]
-lemma default_state_identity_oracle :
-  (identity_oracle spec).default_state = () := rfl
+namespace identity_oracle
 
 @[simp]
 lemma identity_oracle_apply (i : spec.ι) (t : spec.domain i) (s : unit) :
@@ -37,7 +35,7 @@ end
 @[simp]
 lemma support_simulate_identity_oracle_pure (a : A) (s : unit) :
   (simulate idₛ (pure a : oracle_comp spec A) s).support = {(a, ())} :=
-support_simulate_stateless_oracle_pure _ a s
+stateless_oracle.support_simulate_pure _ a s
 
 @[simp]
 lemma support_simulate_identity_oracle (oa : oracle_comp spec A) (s : unit) :
@@ -68,10 +66,6 @@ begin
   refine iff.rfl,
 end
 
-end simulate
-
-section simulate'
-
 @[simp]
 lemma support_simulate'_identity_oracle (oa : oracle_comp spec A) (s : unit) :
   (simulate' idₛ oa s).support = oa.support :=
@@ -83,4 +77,12 @@ begin
   refine ⟨λ h, h.rec_on (λ _ h, h), λ h, ⟨(), h⟩⟩,
 end
 
-end simulate'
+end simulate
+
+section eval_distribution
+
+
+
+end eval_distribution
+
+end identity_oracle
