src/computational_monads/simulation_semantics/constructions/logging/random_oracle.lean
@@ -5,14 +5,29 @@ import computational_monads.simulation_semantics.oracle_compose
 open oracle_comp oracle_spec
 
 variables {spec spec' spec'' : oracle_spec} {A B C : Type}
-  (log : query_log spec) (log' : query_log spec')
 
 /-- Oracle that responds uniformly at random to any new queries,
   but returns the same result to subsequent oracle queries -/
+@[simps]
 noncomputable def random_oracle (spec : oracle_spec) [spec.computable] [spec.finite_range] :
   simulation_oracle spec uniform_selecting :=
 (uniform_oracle spec) ∘ₛ (caching_oracle spec)
 
-@[simp]
-lemma default_state_random_oracle (spec : oracle_spec) [spec.computable] [spec.finite_range] :
-  (random_oracle spec).default_state = (query_log.init spec, ()) := rfl
+namespace random_oracle
+
+variables (log : query_log spec) (log' : query_log spec')
+variable [spec.computable]
+variable [spec.finite_range]
+
+section simulate
+
+
+end simulate
+
+section eval_distribution
+
+
+end eval_distribution
+
+
+end random_oracle
