src/computational_monads/simulation_semantics/constructions/stateless_oracle.lean
@@ -3,11 +3,11 @@ import computational_monads.simulation_semantics.constructions.tracking_oracle
 open oracle_comp oracle_spec
 
 variables {A B : Type} {spec spec' spec'' : oracle_spec}
-  (oa : oracle_comp spec A)
 
 /-- Simulate a computation without making use of the internal state.
   We use the `unit` type as the state in this case, so all possible states are equal.
   Implemented as a `tracking_oracle` where the state isn't actually tracking anything -/
+@[simps]
 def stateless_oracle (spec spec' : oracle_spec)
   (o : Π (i : spec.ι), spec.domain i → oracle_comp spec' (spec.range i)) :
   simulation_oracle spec spec' :=
@@ -15,29 +15,25 @@ def stateless_oracle (spec spec' : oracle_spec)
 
 notation `⟪` o `⟫` := stateless_oracle _ _ o
 
+namespace stateless_oracle
+
+variables (oa : oracle_comp spec A)
+
 variables (o : Π (i : spec.ι), spec.domain i → oracle_comp spec' (spec.range i))
   (o' : Π (i : spec.ι), spec.domain i → oracle_comp spec'' (spec.range i))
 
 @[simp]
-lemma S_stateless_oracle :
-  ⟪o⟫.S = unit := rfl
-
-@[simp]
-lemma default_state_stateless_oracle :
-  ⟪o⟫.default_state = () := rfl
-
-@[simp]
-lemma stateless_oracle_apply (i : spec.ι) (t : spec.domain i) (s : unit) :
+lemma apply (i : spec.ι) (t : spec.domain i) (s : unit) :
   ⟪o⟫.o i (t, s) = o i t >>= λ u, return (u, ()) := rfl
 
 section simulate
 
 @[simp]
-lemma support_simulate_stateless_oracle_pure (a : A) (s : unit) :
+lemma support_simulate_pure (a : A) (s : unit) :
   (simulate ⟪o⟫ (pure a) s).support = {(a, ())} := by simp [punit_eq s ()]
 
 @[simp]
-lemma support_simulate_stateless_oracle_bind (oa : oracle_comp spec A)
+lemma support_simulate_bind (oa : oracle_comp spec A)
   (ob : A → oracle_comp spec B) (s : unit) :
   (simulate ⟪o⟫ (oa >>= ob) s).support =
     ⋃ (x : A × unit) (hx : x ∈ (simulate ⟪o⟫ oa ()).support),
@@ -50,7 +46,7 @@ begin
 end
 
 @[simp]
-lemma support_simulate_stateless_oracle_query (i : spec.ι) (t : spec.domain i) (s : unit) :
+lemma support_simulate_query (i : spec.ι) (t : spec.domain i) (s : unit) :
   (simulate ⟪o⟫ (query i t) s).support = {x | x.1 ∈ (o i t).support} :=
 begin
   refine s.rec _,
@@ -62,7 +58,7 @@ end simulate
 
 section eval_distribution
 
-lemma simulate_stateless_oracle_equiv_simulate' [spec'.finite_range] (s : unit) :
+lemma simulate_equiv_simulate' [spec'.finite_range] (s : unit) :
   simulate ⟪o⟫ oa s ≃ₚ (simulate' ⟪o⟫ oa s >>= λ a, pure (a, ())) :=
 calc simulate ⟪o⟫ oa s ≃ₚ simulate ⟪o⟫ oa s >>= pure : symm (bind_pure_equiv _)
   ... ≃ₚ simulate ⟪o⟫ oa s >>= λ x, pure (x.1, x.2) : by simp only [prod.mk.eta]
@@ -70,7 +66,7 @@ calc simulate ⟪o⟫ oa s ≃ₚ simulate ⟪o⟫ oa s >>= pure : symm (bind_pu
     bind_equiv_of_equiv_second _ (λ x, by simp [punit_eq x.snd ()])
   ... ≃ₚ simulate' ⟪o⟫ oa s >>= λ a, pure (a, ()) : by rw [simulate', bind_map_equiv]
 
-lemma simulate'_stateless_oracle_equiv_of_oracle_equiv [spec'.finite_range] [spec''.finite_range] 
+lemma simulate'_equiv_of_oracle_equiv [spec'.finite_range] [spec''.finite_range] 
   {o : Π (i : spec.ι), spec.domain i → oracle_comp spec' (spec.range i)}
   {o' : Π (i : spec.ι), spec.domain i → oracle_comp spec'' (spec.range i)}
   (s : unit) (h : ∀ (i : spec.ι) (t : spec.domain i), o i t ≃ₚ o' i t) :
@@ -81,24 +77,26 @@ begin
   { calc simulate' ⟪o⟫ (oa >>= ob) s
       ≃ₚ simulate ⟪o⟫ oa s >>= λ x, simulate' ⟪o⟫ (ob x.1) x.2 : simulate'_bind_equiv ⟪o⟫ oa ob _
       ... ≃ₚ simulate ⟪o'⟫ oa s >>= λ x, simulate' ⟪o'⟫ (ob x.1) x.2 : begin
-        simp [simulate_stateless_oracle_equiv_simulate', hoa],
+        simp [simulate_equiv_simulate', hoa],
         congr,
         simpa [hob],
       end
       ... ≃ₚ simulate' ⟪o'⟫ (oa >>= ob) s : symm (simulate'_bind_equiv ⟪o'⟫ oa ob _) },
-  { simp_rw [simulate'_query_equiv, stateless_oracle_apply, fst_map_bind_mk_equiv],
+  { simp_rw [simulate'_query_equiv, stateless_oracle.apply, fst_map_bind_mk_equiv],
     exact map_equiv_of_equiv _ _ id (h i t) }
 end 
 
-lemma simulate'_stateless_oracle_query_equiv [spec.finite_range] (s : unit) :
+lemma simulate'_query_equiv [spec.finite_range] (s : unit) :
   simulate' ⟪query⟫ oa s ≃ₚ oa :=
-simulate'_tracking_oracle_query_equiv _ _ _ _
+tracking_oracle.simulate'_query_equiv _ _ _ _
 
-lemma simulate'_stateless_oracle_query_equiv_of_equiv [spec.finite_range] [spec'.finite_range] (s : unit)
+lemma simulate'_query_equiv_of_equiv [spec.finite_range] [spec'.finite_range] (s : unit)
   (ho : ∀ (i : spec.ι) (t : spec.domain i), o i t ≃ₚ query i t) :
   simulate' ⟪o⟫ oa s ≃ₚ oa :=
 calc simulate' ⟪o⟫ oa s ≃ₚ simulate' ⟪query⟫ oa s
-    : simulate'_stateless_oracle_equiv_of_oracle_equiv oa s ho
-  ... ≃ₚ oa : simulate'_stateless_oracle_query_equiv oa s
+    : simulate'_equiv_of_oracle_equiv oa s ho
+  ... ≃ₚ oa : simulate'_query_equiv oa s
 
 end eval_distribution
+
+end stateless_oracle
