src/computational_monads/simulation_semantics/constructions/uniform_oracle.lean
@@ -4,16 +4,28 @@ import computational_monads.constructions.uniform_select
 open oracle_comp oracle_spec
 
 variables {A B : Type} {spec spec' spec'' : oracle_spec}
-  (oa : oracle_comp spec A)
 
+@[simps]
 noncomputable def uniform_oracle (spec : oracle_spec) [spec.finite_range] : 
   simulation_oracle spec uniform_selecting :=
 ⟪ λ i t, $ᵗ (spec.range i) ⟫
 
-@[simp]
-lemma default_state_uniform_oracle (spec : oracle_spec) [spec.finite_range] :
-  (uniform_oracle spec).default_state = () := rfl
+namespace uniform_oracle
+
+variables (oa : oracle_comp spec A)
 
 @[simp]
 lemma uniform_oracle_apply (spec : oracle_spec) (i : spec.ι) (t : spec.domain i) [spec.finite_range] (s : unit) :
   (uniform_oracle spec).o i (t, s) = $ᵗ (spec.range i) >>= λ u, return (u, ()) := rfl
+
+section simulate
+
+
+end simulate
+
+section eval_distribution
+
+
+end eval_distribution
+
+end uniform_oracle
